---
title: "CBowersox_Assign14"
author: "Cheryl Bowersox"
date: "Saturday, May 09, 2015"
output: pdf_document
---
## Taylor Series expansions

### function:  $f(x) = \frac{1}{1-x} x\in(-1,1)$

$$
  f(x) = (1-x)^{-1}\\    
  f'(x) = (1-x)^{-2}\\
  f''(x) = 2(1-x)^{-3}\\
  f'''(x) = 6(1-x)^{-4}\\
  ...\\
  f^{(n)}(x) = n!(1-x)^{-(n+1)}\\
$$

$$
  a = 0\\
  f(a) = 1\\
  f'(a) = 1\\
  f''(a) = 2\\
  f'''(a) = 6\\
  ...\\
  f^{(n)}(a) = n!\\
$$

$$
  f(x) = \sum_{n=0}^{\infty} \frac{f^{(n)}(a)}{n!}(x - a)^{n}\\
  a = 0:\\
  f(x) = \sum_{n=0}^{\infty} \frac{n!}{n!}(x - 0)^{n}\\
  f(x) = \sum_{n=0}^{\infty} x^{n}\\
$$
  in general $a \in (-1,1) \\$
$$
  f(x) = \sum_{n=0}^{\infty} \frac{n!(1-a)^{-(n+1)}}{n!}(x - a)^{n}\\
  f(x) = \sum_{n=0}^{\infty} \frac{(x-a)^{n}}{(1-a)^{n+1}}
$$


### function: $f(x) = e^{x}$

$$
  f(x) = e^{x}\\    
  f'(x) = e^{x}\\
  f''(x) = e^{x}\\
  f'''(x) = e^{x} \\
  ...\\
  f^{(n)}(x) = e^x\\
$$

$$
  a = 0\\
  f(a) = 1\\
  f'(a) = 1\\
  f''(a) = 1\\
  f'''(a) = 1\\
  ...\\
  f^{(n)}(a) = 1\\
$$

$$
  f(x) = \sum_{n=0}^{\infty} \frac{f^{(n)}(a)}{n!}(x - a)^{n}\\
  f(x) = \sum_{n=0}^{\infty} \frac{1}{n!}(x - 0)^{n}\\
  f(x) = \sum_{n=0}^{\infty} \frac{x^{n}}{n!}\\
$$
  in general $a \in R \\$
$$
  f(x) = \sum_{n=0}^{\infty} \frac{e^a}{n!}(x - a)^{n}\\
$$



### function:  $f(x) = ln(1+x) x\in(-1,1)$

$$
  f(x) = ln(1+x)\\
  f'(x) = (1+x)^{-1}\\
  f''(x) = -(1+x)^{-2}\\
  f'''(x) = 2(1+x)^{-3} \\
  f^{(4)}(x) = -6(1+x)x^{-4} \\
  ...\\
  f^{(n)}(x) = -1^{n+1}(n-1)!(1+x)^{-n},  n>0\\
$$

$$
  a = 0\\
  f(a) = 0\\   
  f'(a) = 1\\
  f''(a) = -1\\
  f'''(a) = 2\\
  f'''(a) = -6\\
  ...\\
  f^{(n)}(a) = -1^{n+1}(n-1)!,  n>0\\
$$

$$
  f(x) = \sum_{n=1}^{\infty} \frac{f^{(n)}(a)}{n!}(x - a)^{n}\\
  f(x) = \sum_{n=1}^{\infty} \frac{-1^{n+1}(n-1)!}{n!}(x - 0)^{n}\\
  f(x) = \sum_{n=1}^{\infty} \frac{-1^{n+1}x^{n}}{n}\\
$$

in general $a \in (-1,1) \\$

$$
  f(x) = ln(1+a) + \sum_{n=1}^{\infty} \frac{-1^{n-1}(1+a)^{-n}}{n}(x - a)^{n}\\
$$
